proofs/fstar/extraction/Sandwich.Tunnel.Tls.Security.fst
@@ -13,7 +13,11 @@ let assert_tls13_compliance = assert_tls13_compliance'
 /// Checks that the policy is satisfied by the configuration.
 let assert_compliance (cfg: Sandwich_api_proto.Configuration.t_Configuration)
     : Core.Result.t_Result Prims.unit Sandwich.Error.t_Error =
-  match Sandwich.Tunnel.Tls.get_tls13_config cfg with
+  match
+    Sandwich.Tunnel.Tls.get_tls13_config cfg
+    <:
+    Core.Option.t_Option Sandwich_api_proto.Tls.t_TLSv13Config
+  with
   | Core.Option.Option_Some tls13 -> assert_tls13_compliance tls13
   | _ ->
     Core.Result.Result_Ok (() <: Prims.unit)
